src/program_proof/simplepb/pb_becomeprimary_proof.v
@@ -28,7 +28,7 @@ Lemma wp_Clerk__BecomePrimary γ γsrv ck args_ptr args σ backupγ:
         "#Hepoch_lb" ∷ is_epoch_lb γsrv.(r_pb) args.(BecomePrimaryArgs.epoch) ∗
         "#Hconf" ∷ is_epoch_config γ.(s_pb) args.(BecomePrimaryArgs.epoch) (r_pb <$> γsrv :: backupγ) ∗
         "#Hhosts" ∷ ([∗ list] host ; γsrv' ∈ args.(BecomePrimaryArgs.replicas) ; γsrv :: backupγ,
-                       is_pb_host host γ γsrv' ∗
+                       is_pb_rpcs host γ γsrv' ∗
                        is_epoch_lb γsrv'.(r_pb) args.(BecomePrimaryArgs.epoch)) ∗
         "#Hprim_escrow" ∷ become_primary_escrow γ.(s_prim) γsrv.(r_prim) args.(BecomePrimaryArgs.epoch) σ
                           (own_primary_ghost γ.(s_pb) args.(BecomePrimaryArgs.epoch) σ) ∗
@@ -53,7 +53,7 @@ Proof.
   wp_loadField.
   iDestruct (own_slice_to_small with "Henc_args_sl") as "Henc_args_sl".
   wp_apply (wp_frame_wand with "HΦ").
-  rewrite is_pb_host_unfold.
+  rewrite is_pb_rpcs_unfold.
   iNamed "Hsrv".
   wp_apply (wp_ReconnectingClient__Call2 with "Hcl_rpc [] Henc_args_sl Hrep").
   {
@@ -104,7 +104,7 @@ Lemma become_primary_eph_step γ γsrv st σ backupγ replicaHosts:
   is_proposal_facts_prim γ.(s_prim) st.(server.epoch) σ -∗
   is_epoch_config γ.(s_pb) st.(server.epoch) (r_pb <$> γsrv :: backupγ) -∗
   ([∗ list] host ; γsrv' ∈ replicaHosts ; γsrv :: backupγ,
-                  is_pb_host host γ γsrv' ∗
+                  is_pb_rpcs host γ γsrv' ∗
                   is_epoch_lb γsrv'.(r_pb) st.(server.epoch)) -∗
   become_primary_escrow γ.(s_prim) γsrv.(r_prim) st.(server.epoch) σ
                     (own_primary_ghost γ.(s_pb) st.(server.epoch) σ) -∗
@@ -135,7 +135,7 @@ Lemma wp_Server__BecomePrimary γ γsrv s args_ptr args σ backupγ Φ Ψ :
   is_Server s γ γsrv -∗
   BecomePrimaryArgs.own args_ptr args -∗
   (∀ (err:u64), Ψ err -∗ Φ #err) -∗
-  BecomePrimary_core_spec γ γsrv args σ backupγ is_pb_host Ψ -∗
+  BecomePrimary_core_spec γ γsrv args σ backupγ is_pb_rpcs Ψ -∗
   WP pb.Server__BecomePrimary #s #args_ptr {{ Φ }}
   .
 Proof.
